\documentclass[a4paper]{article}
\usepackage{a4wide}
\usepackage{amsmath}
\usepackage{amssymb}
\usepackage{dsfont}
\pagestyle{plain}
\usepackage{tikz}
\usetikzlibrary{matrix}
\usepackage{eurosym}
\usepackage{amsthm}
\usepackage{mathrsfs}
\usepackage{dlfltxbcodetips}

\begin{document}
\section*{Exercise 1a}
\begin{align*}
\frac{\partial C}{\partial q_i}
&=\frac{\partial}{\partial q_i}\sum_{j}p_j\log(\frac{p_j}{q_j})\\
&=\sum_{j}\frac{\partial}{\partial q_i}\left(p_j\log(\frac{p_j}{q_j})\right)\\
&=\sum_{j}\frac{\partial}{\partial q_i}\left(p_j\log(p_j)-p_jlog(q_j)\right)\\
&=\sum_{j}\left(-p_j\frac{\partial}{\partial q_i}log(q_j)\right)\\
\end{align*}
Since \[ \frac{\partial}{\partial q_i}log(q_j)=\begin{cases}
   0 &, i\neq j \\
   \frac{1}{q_i} &, i=j\end{cases},  \]
\begin{align*}
\frac{\partial C}{\partial q_i}
&=-\frac{p_i}{q_i}.\\
\end{align*}
\section*{Exercise 1b}
\begin{align*}
\frac{\partial C}{\partial x_i}
&=\frac{\partial}{\partial x_i}\sum_{j}p_j\log(\frac{p_j}{q_j})\\
&=\sum_{j}\frac{\partial}{\partial x_i}\left(p_j\log(p_j)-p_jlog(q_j)\right)\\
&=\sum_{j}\left(-p_j\frac{\partial}{\partial x_i}log(q_j)\right)\\
&=\sum_{j}\left(-p_j\frac{\partial}{\partial x_i}log(\frac{e^{x_j}}{\sum_{k}e^{x_k}})\right)\\
&=\sum_{j}\left(-p_j\frac{\partial}{\partial x_i}(x_j-log(\sum_{k}e^{x_k}))\right)\\
&=\sum_{j}\left(-p_j\frac{\partial}{\partial x_i}x_j\right)+\sum_{j}\left(p_j\frac{\partial}{\partial x_i}log(\sum_{k}e^{x_k})\right)\\
&=\sum_{j}\left(-p_j\frac{\partial}{\partial x_i}x_j\right)+\sum_{j}\left(p_j\frac{1}{\sum_{k}e^{x_k}}\frac{\partial}{\partial x_i}\sum_{k}e^{x_k}\right)\\
&=\sum_{j}\left(-p_j\frac{\partial}{\partial x_i}x_j\right)+\sum_{j}\left(p_j\frac{e^{x_i}}{\sum_{k}e^{x_k}}\right)\\
&=\sum_{j}\left(-p_j\frac{\partial}{\partial x_i}x_j\right)+q_i\sum_{j}p_j\\
&=\sum_{j}\left(-p_j\frac{\partial}{\partial x_i}x_j\right)+q_i\\
\end{align*}
Since \[ \frac{\partial}{\partial x_i}x_j=\begin{cases}
   0 &, i\neq j \\
   1 &, i=j\end{cases},  \]
\begin{align*}
\frac{\partial C}{\partial x_i}
&=-p_i+q_i\\
\end{align*}
\end{document}